Use generic list class to replace open-coded helpers

CPPSynth/Generate.v
@@ -10,6 +10,7 @@ Require Import
   CPPSynth.Gallina
   CPPSynth.CPPAst
   CPPSynth.CPPAstVisit
+  CPPSynth.ListClass
   CPPSynth.Monad.
 
 Module cg.
@@ -32,15 +33,15 @@ Module cg.
   Definition move_of (expr : expr_t) : expr_t :=
     expr_call
       (expr_id (idexpr_id (scope_id "std" scope_none) "move"))
-      (make_callargs (expr :: nil)).
+      (from_list (expr :: nil)).
   Definition make_shared_of (type : typeexpr_t) (args : list expr_t) :=
     expr_call
       (expr_id (
         idexpr_template (scope_id "std" scope_none) (templateid_make "make_shared"
           (tplargs_cons (tplarg_type type) tplargs_nil))))
-      (make_callargs args).
+      (from_list args).
   Definition fn_type (result_type : typeexpr_t) (args : list (option string * typeexpr_t)) : typeexpr_t :=
-    let fnargs := make_funargs (map (fun (a : option string * typeexpr_t) => let (name, type) := a in
+    let fnargs := from_list (map (fun (a : option string * typeexpr_t) => let (name, type) := a in
       match name with
         | None => funarg_anon type
         | Some n => funarg_named type n
@@ -51,589 +52,22 @@ Module cg.
     let std_logic_error :=
       expr_id (idexpr_id (scope_id "std" scope_none) "logic_error") in
     let arg := expr_literal (literal.str msg) in
-    expr_throw (expr_call std_logic_error (make_callargs (arg :: nil))).
+    expr_throw (expr_call std_logic_error (from_list (arg :: nil))).
   Definition deleted_constructor (name : string) (args : list funarg_t): decl_t :=
     decl_consdesdef
       declspec.none
       (idexpr_id scope_none name)
-      (make_funargs args)
+      (from_list args)
       fnqual.none
       attrspec.none
       funbody_delete.
 End cg.
-
-Fixpoint make_tplargs (args : list tplarg_t) : tplargs_t :=
-  match args with
-    | nil => tplargs_nil
-    | arg :: args => tplargs_cons arg (make_tplargs args)
-  end.
-
-Fixpoint make_tplformargs (args : list tplformarg_t) : tplformargs_t :=
-  match args with
-    | nil => tplformargs_nil
-    | arg :: args => tplformargs_cons arg (make_tplformargs args)
-  end.
-
-Module env.
-  Inductive t : Set :=
-    | empty : t.
-
-  Fixpoint to_type (e : expr.t) (this : t) : typeexpr_t :=
-    match e with
-      | expr.global n => cg.named_type n
-      | expr.local n _ => cg.named_type n
-      | expr.app fn arg =>
-        to_type_template_apply fn ((to_type arg this) :: nil) this
-      | expr.product argname argtype body =>
-        to_type_fn_abstract ((argname, to_type argtype this) :: nil) body this
-    end
-  with to_type_template_apply (fn : expr.t) (args : list typeexpr_t) (this : t) : typeexpr_t :=
-    match fn with
-      | expr.global n =>
-        let tplargs := make_tplargs (map (fun arg => tplarg_type arg) args) in
-        typeexpr_id (idexpr_template scope_none (templateid_make n tplargs))
-      | expr.app fn arg =>
-        to_type_template_apply fn (args ++ (to_type arg this) :: nil) this
-      | _ => typeexpr_primitive (primtype.auto)
-    end
-  with to_type_fn_abstract (args : list (option string * typeexpr_t)) (body : expr.t) (this : t) : typeexpr_t :=
-    match body with
-      | expr.product argname argtype body =>
-        to_type_fn_abstract (args ++ ((argname, to_type argtype this) :: nil)) body this
-      | expr.global n =>
-        let result_type := cg.named_type n in
-        cg.fn_type result_type args
-      | expr.local n _ =>
-        let result_type := cg.named_type n in
-        cg.fn_type result_type args
-      | expr.app fn arg =>
-        let result_type := to_type_template_apply fn ((to_type arg this) :: nil) this in
-        cg.fn_type result_type args
-    end.
-  Definition to_tplformarg (name : string) (e : expr.t) (this : t) : tplformarg_t :=
-    match e with
-      | expr.global ename =>
-        if string_dec ename "Set" then
-          tplformarg_typename name
-        else if string_dec ename "Type" then
-          tplformarg_typename name
-        else
-          tplformarg_value (to_type e this) name
-      | _ => tplformarg_value (to_type e this) name
-    end.
-End env.
-
-Definition product_unfold (e : expr.t) : list (option string * expr.t) * expr.t :=
-  let head := nil in
-  (fix loop (e : expr.t) (head : list (option string * expr.t))
-      : list (option string * expr.t) * expr.t :=
-    match e with
-      | expr.product argname argtype body =>
-        let head := head ++ (argname, argtype) :: nil in
-        loop body head
-      | _ =>
-        (head, e)
-    end) e head.
-
-(* make choice of prefix name configurable *)
-Definition product_named_unfold (e : expr.t) : list (string * expr.t) * expr.t :=
-  let head := nil in
-  let index := 0 in
-  (fix loop (e : expr.t) (index : nat) (head : list (string * expr.t))
-      : list (string * expr.t) * expr.t :=
-    match e with
-      | expr.product argname argtype body =>
-        let name :=
-          match argname with
-            | Some name => name
-            | None => ("x" ++ (string_of_nat index))%string
-          end in
-        let head := head ++ (name, argtype) :: nil in
-        loop body (S index) head
-      | _ =>
-        (head, e)
-    end) e index head.
-
-Fixpoint collect_tplformargs_from_product
-    (e : expr.t) : tplformargs_t :=
-  match e with
-    | expr.product maybe_name argtype body =>
-      let name :=
-        match maybe_name with
-          | Some name => name
-          | None => "T"%string
-        end in
-      tplformargs_cons (tplformarg_typename name) (collect_tplformargs_from_product body)
-    | _ => tplformargs_nil
-  end.
 
 Definition maybe_template (tpl : tplformargs_t) (d : decl_t) : decl_t :=
   match tpl with
     | tplformargs_nil => d
     | _ => decl_templated tpl d
   end.
-
-Definition one_inductive_fwd (oi : one_inductive.t) : decl_t :=
-  let (name, sig, constructors) := oi in
-  let tpl := collect_tplformargs_from_product sig in
-  let d := decl_class_fwd (idexpr_id scope_none name) in
-  maybe_template tpl d.
-
-Definition inductive_fwd (i : inductive.t) : list decl_t :=
-  let (ois) := i in
-  map (one_inductive_fwd) ois.
-
-Definition gen_virtual_destructor_decldef (name : string) : decl_t :=
-  let ds := declspec.none in
-  let ds := declspec.set_virtual ds in
-  decl_consdesdef
-    ds
-    (idexpr_destructor scope_none name)
-    (make_funargs nil)
-    fnqual.none
-    attrspec.none
-    (funbody_stmts cinits_nil (make_stmts nil)).
-
-Definition make_repr_base_class (name : string) :=
-  let repr_cls_type := typeexpr_id (idexpr_id scope_none name) in
-  let eq_operator :=
-    decl_fundef
-      (declspec.set_virtual declspec.none)
-      (funtypeexpr_make
-        (typeexpr_primitive primtype.bool)
-        (make_funargs (funarg_named (cg.constref_of repr_cls_type) "other" :: nil))
-        (fnqual.set_noexcept (fnqual.set_const fnqual.none))
-        false)
-      (idexpr_operator scope_none (overloadable_operator.binary binop.eq))
-      attrspec.none
-      funbody_abstract in
-  decl_class
-    (idexpr_id scope_none name)
-    false
-    clsinherits_nil
-    (clsdecls_cons
-      (clsdecl_group
-        visibility_spec.vis_public
-        (make_decls
-          (gen_virtual_destructor_decldef name ::
-          eq_operator ::
-          nil)))
-      clsdecls_nil).
-
-Definition constructor_reprclass_name (cons : inductive_constructor.t) : string :=
-  ((inductive_constructor.name cons) ++ "_repr").
-
-Definition constructor_reprclass_members (cons : inductive_constructor.t)
-    : list (string * expr.t) :=
-  fst (product_named_unfold (inductive_constructor.type cons)).
-
-Fixpoint make_cinits (is : list cinit_t)
-    : cinits_t :=
-  match is with
-    | nil => cinits_nil
-    | cons i is => cinits_cons i (make_cinits is)
-  end.
-
-Definition make_constructor_repr_class
-    (cons : inductive_constructor.t)
-    (environ : env.t) :=
-  let name := constructor_reprclass_name cons in
-  let members := constructor_reprclass_members cons in
-
-  let repr_cls_id := idexpr_id scope_none name in
-  let repr_cls_type := typeexpr_id repr_cls_id in
-  let repr_constptr := typeexpr_pointer (typeexpr_const repr_cls_type) in
-
-  let base_cls_id := (idexpr_id scope_none "repr_base") in
-  let base_cls_type := typeexpr_id base_cls_id in
-
-  let member_decls := map
-    (fun (mem : string * expr.t) =>
-      let (name, e) := mem in
-      let type := env.to_type e environ in
-      decl_simple declspec.none type (idexpr_id scope_none name) attrspec.none) members in
-  let init_formal_args := map
-    (fun (mem : string * expr.t) =>
-      let (name, e) := mem in
-      let type := env.to_type e environ in
-      funarg_named type (name ++ "_init")) members in
-  let initializers := map
-    (fun (mem : string * expr.t) =>
-      let (name, e) := mem in
-      cinit_make
-        (idexpr_id scope_none name)
-        (cg.move_of (expr_id (idexpr_id scope_none (name ++ "_init"))))) members in
-  let cls_constructor := decl_consdesdef
-    declspec.none
-    (idexpr_id scope_none name)
-    (make_funargs init_formal_args)
-    fnqual.none
-    attrspec.none
-    (funbody_stmts
-      (make_cinits initializers)
-      stmts_nil) in
-  let overridden_eq_operator :=
-    decl_fundef
-      declspec.none
-      (funtypeexpr_make
-        (typeexpr_primitive primtype.bool)
-        (make_funargs (funarg_named (cg.constref_of base_cls_type) "other" :: nil))
-        (fnqual.set_noexcept (fnqual.set_const fnqual.none))
-        false)
-      (idexpr_operator scope_none (overloadable_operator.binary binop.eq))
-      (attrspec.set_override attrspec.none)
-      (funbody_stmts cinits_nil
-        (make_stmts
-          (stmt_ifelse
-            (condition_decl
-              declspec.none (typeexpr_primitive primtype.auto)
-              (idexpr_id scope_none "spec")
-              attrspec.none
-              (expr_dynamic_cast repr_constptr (expr_unop unop.address_of (expr_id (idexpr_id scope_none "other")))))
-            (stmt_block (make_stmts
-              (stmt_return (expr_binop binop.eq
-                (expr_unop unop.deref (expr_id (idexpr_id scope_none "this")))
-                (expr_unop unop.deref (expr_id (idexpr_id scope_none "spec"))))
-              :: nil)))
-            (stmt_block (make_stmts
-              (stmt_return (expr_id (idexpr_id scope_none "false")) :: nil))) ::
-          nil))) in
-  let member_compare := map
-    (fun (mem : string * expr.t) =>
-      let (name, e) := mem in
-      let id := idexpr_id scope_none name in
-      expr_binop binop.eq (expr_id id) (expr_memdot (expr_id (idexpr_id scope_none "other")) id))
-      members in
-  let all_member_eq := fold_right
-    (fun (x y : expr_t) => expr_binop binop.logic_and x y)
-    (expr_id (idexpr_id scope_none "true")) member_compare in
-  let specialized_eq_operator :=
-    decl_fundef
-      declspec.none
-      (funtypeexpr_make
-        (typeexpr_primitive primtype.bool)
-        (make_funargs (funarg_named (cg.constref_of repr_cls_type) "other" :: nil))
-        (fnqual.set_noexcept (fnqual.set_const fnqual.none))
-        false)
-      (idexpr_operator scope_none (overloadable_operator.binary binop.eq))
-      attrspec.none
-      (funbody_stmts cinits_nil
-        (make_stmts (stmt_return all_member_eq :: nil))) in
-  decl_class
-    repr_cls_id
-    true
-    (clsinherits_cons (clsinherit_single false visibility_spec.vis_public base_cls_id) clsinherits_nil)
-    (make_clsdecls
-      ((clsdecl_group
-        visibility_spec.vis_public
-        (make_decls (cls_constructor :: specialized_eq_operator :: overridden_eq_operator :: member_decls))) :: nil)).
-
-(*
-  Roughly builds the following:
-
-  if (const as_type* temp_name = dynamic_cast<const as_type*>(base_expr)) {
-    call_expr(temp_name->member1, temp_name->member2, ..., temp_name->membern);
-  }
-
-  Returns the "condition" and "body" part of the if statement as a pair.
-
-  Can form the above statement as:
-    stmt_if condition body
-*)
-Definition make_single_match_test
-    (base_expr : expr_t) (as_type : typeexpr_t) (temp_name : idexpr_t)
-    (call_expr : expr_t) (members : list string)
-    : condition_t * stmt_t :=
-  let target_type := cg.constptr_of as_type in
-  let temp_expr := expr_id temp_name in
-  let callargs :=
-    map
-      (fun member =>
-        expr_memarrow (expr_id temp_name) (idexpr_id scope_none member))
-      members in
-  let cond := (condition_decl
-      declspec.none (cg.type_auto) temp_name attrspec.none
-      (expr_dynamic_cast target_type base_expr)) in
-  let body :=
-    stmt_block (
-      make_stmts
-        ((stmt_return (expr_call call_expr (make_callargs callargs))) :: nil)) in
-  (cond, body).
-
-(*
-  Produce a statement that checks 'base_expr' with match for any of the
-  constructor repr classes (via dynamic_cast) and dispatches to the
-  corresponding call expression.
-*)
-Fixpoint make_match_constructors
-    (base_expr : expr_t) (branches : list (inductive_constructor.t * expr_t))
-    : stmt_t :=
-  match branches with
-    | nil => stmt_block (make_stmts (stmt_expr (cg.throw_logic_error "impossible case" ) :: nil))
-    | branch :: branches =>
-      let sub := make_match_constructors base_expr branches in
-      let (cons, call_expr) := branch in
-      let cons_name := constructor_reprclass_name cons in
-      let cons_members := constructor_reprclass_members cons in
-      let member_names := map fst cons_members in
-      let as_type := typeexpr_id (idexpr_id scope_none cons_name) in
-      let temp_name := idexpr_id scope_none "tmp" in
-      let (cond, body) := make_single_match_test base_expr as_type temp_name call_expr member_names in
-      stmt_ifelse cond body sub
-  end.
-
-Definition make_name_type_pairs (args : list (option string * expr.t)) (environ : env.t)
-    : list (string * typeexpr_t) :=
-  map
-    (fun (ca : option string * expr.t) =>
-      let (n, e) := ca in
-      let type := env.to_type e environ in
-      let name := match n with
-        | Some n => n
-        | None => "_"%string
-      end in
-      (name, type))
-    args.
-
-Definition make_match_fntype
-    (constructors : list inductive_constructor.t)
-    (environ : env.t) : (list tplformarg_t) * funtypeexpr_t :=
-  (* special case for empty inductive type (not useful, but...) *)
-  match constructors with
-    | first_constructor :: _ =>
-      (* collect names of all constructors *)
-      let consnames := map inductive_constructor.name constructors in
-      (* template argument list for match handler functionals *)
-      let tplargs := map (fun name => tplformarg_typename ("F" ++ name)%string) consnames in
-      (* the formal arguments of our "match" function *)
-      let formal_args :=
-        make_funargs (
-          map
-            (fun name =>
-             funarg_named
-              (cg.constref_of (cg.named_type ("F" ++ name)))
-              ("f" ++ name))
-            consnames) in
-      (* arguments to first constructor *)
-      let pre_callargs := fst (product_unfold (inductive_constructor.type first_constructor)) in
-      (* turn them into "declval" constructs *)
-      let callargs := map (fun (ca : option string * expr.t) =>
-        let (_, e) := ca in
-        let type := env.to_type e environ in
-        cg.declval_of (cg.constref_of type)) pre_callargs in
-      let ret_type :=
-        typeexpr_decltype (expr_call (expr_id (idexpr_id scope_none ("F" ++ (inductive_constructor.name first_constructor)))) (make_callargs callargs)) in
-      (tplargs, funtypeexpr_make ret_type formal_args fnqual.none true)
-    | nil =>
-      (nil, funtypeexpr_make (typeexpr_primitive primtype.void) funargs_nil fnqual.none false)
-  end.
-
-Definition make_inductive_cons_factory_fn
-    (ind_clsname : string) (consname : string) (cons_args : list (string * expr.t))
-    : decl_t :=
-  let environ := env.empty in
-  let formal_args :=
-    map
-      (fun (c : string * expr.t) =>
-        let (name, e) := c in
-        funarg_named (env.to_type e environ) name)
-      cons_args in
-  let args :=
-    map
-      (fun (c : string * expr.t) =>
-        let (name, e) := c in
-        cg.move_of (expr_id (idexpr_id scope_none name)))
-      cons_args in
-  let fntype :=
-    funtypeexpr_make
-      (cg.named_type ind_clsname)
-      (make_funargs formal_args)
-      fnqual.none
-      false in
-  let repr_instance :=
-    cg.make_shared_of
-      (cg.named_type (consname ++ "_repr"))
-      args in
-  let cls_instance :=
-    expr_call (expr_id (idexpr_id scope_none ind_clsname)) (make_callargs (repr_instance :: nil)) in
-  decl_fundef
-    (declspec.set_static declspec.none)
-    fntype
-    (idexpr_id scope_none consname)
-    attrspec.none
-    (funbody_stmts
-      cinits_nil
-      (make_stmts (stmt_return cls_instance :: nil))).
-
-Definition one_inductive_decl_parts (oi : one_inductive.t)
-    : tplformargs_t * idexpr_t * clsdecls_t :=
-  let environ := env.empty in
-  let (name, sig, constructors) := oi in
-
-  (* names of the inductive constructors *)
-  let consnames := map (fun (c : inductive_constructor.t) => let (name, _) := c in name) constructors in
-
-  (* template arguments, in case this is a parameterized inductive type *)
-  let tpl := collect_tplformargs_from_product sig in
-
-  (* the C++ class name... *)
-  let cls_name := name in
-  let cls_id := idexpr_id scope_none cls_name in
-  let cls_type := typeexpr_id cls_id in
-
-  (* the repr_ member id *)
-  let id_repr_m := (idexpr_id scope_none "repr_") in
-
-  (* internal base representation class, abstract *)
-  let repr_base_class_def := make_repr_base_class "repr_base" in
-  let repr_ptr_type := (cg.shared_ptr_of (cg.named_type "repr_base")) in
-
-  (* internal representation classes, to represent the different
-  inductive constructors *)
-  let repr_classes := map (fun c => make_constructor_repr_class c environ) constructors in
-
-  (* match function to discriminate between the different constructors *)
-  let (match_fn_tplargs, match_fn_type) := make_match_fntype constructors environ in
-  let cons_call := map
-    (fun (cons : inductive_constructor.t) =>
-      (cons, expr_id (idexpr_id scope_none ("f" ++ inductive_constructor.name cons)))) constructors in
-  let match_fn_decl :=
-    decl_fundef
-      declspec.none
-      match_fn_type
-      (idexpr_id scope_none "match")
-      attrspec.none
-      (funbody_stmts
-        cinits_nil
-        (make_stmts
-          (make_match_constructors (expr_id id_repr_m) cons_call :: nil))) in
-  let match_fn_tpldecl := maybe_template (make_tplformargs match_fn_tplargs) match_fn_decl in
-
-  (* The static factory functions to create instances of this object
-  per each inductive constructor. *)
-  let factory_fns :=
-    map
-      (fun (cons : inductive_constructor.t) =>
-        let (consname, _) := cons in
-        let members := constructor_reprclass_members cons in
-        make_inductive_cons_factory_fn cls_name consname members
-      )
-      constructors in
-
-  (* C++ class constructors *)
-  let primary_constructor :=
-    decl_consdesdef
-      (declspec.set_explicit declspec.none)
-      cls_id
-      (make_funargs ((funarg_named repr_ptr_type "repr") :: nil))
-      (fnqual.set_noexcept fnqual.none)
-      attrspec.none
-      (funbody_stmts
-        (cinits_cons (cinit_make (idexpr_id scope_none "repr_") (cg.move_of (expr_id (idexpr_id scope_none "repr")))) cinits_nil)
-        (make_stmts nil)) in
-  let copy_constructor :=
-    decl_consdesdef
-      declspec.none
-      cls_id
-      (make_funargs (((funarg_named (cg.constref_of cls_type) "other")) :: nil))
-      (fnqual.set_noexcept fnqual.none)
-      attrspec.none
-      funbody_default in
-  let move_constructor :=
-    decl_consdesdef
-      declspec.none
-      cls_id
-      (make_funargs (((funarg_named (typeexpr_rvaluereference cls_type) "other")) :: nil))
-      (fnqual.set_noexcept fnqual.none)
-      attrspec.none
-      funbody_default in
-  let default_constructor := cg.deleted_constructor cls_name nil in
-
-  let assign_operator :=
-    decl_fundef
-      declspec.none
-      (funtypeexpr_make
-        (typeexpr_reference cls_type)
-        (make_funargs (funarg_named (cg.constref_of cls_type) "other" :: nil))
-        (fnqual.set_noexcept fnqual.none)
-        false)
-      (idexpr_operator scope_none (overloadable_operator.binary binop.assign))
-      attrspec.none
-      (funbody_stmts
-        cinits_nil
-        (make_stmts (
-          stmt_expr (expr_binop binop.assign (expr_id id_repr_m)
-            (expr_memarrow (expr_id (idexpr_id scope_none "other")) id_repr_m)) ::
-          stmt_return (expr_unop unop.deref (expr_id (idexpr_id scope_none "this"))) ::
-          nil))) in
-
-  let assign_move_operator :=
-    decl_fundef
-      declspec.none
-      (funtypeexpr_make
-        (typeexpr_reference cls_type)
-        (make_funargs (funarg_named (typeexpr_rvaluereference cls_type) "other" :: nil))
-        (fnqual.set_noexcept fnqual.none)
-        false)
-      (idexpr_operator scope_none (overloadable_operator.binary binop.assign))
-      attrspec.none
-      (funbody_stmts
-        cinits_nil
-        (make_stmts (
-          stmt_expr (expr_binop binop.assign (expr_id id_repr_m)
-            (cg.move_of (expr_memarrow (expr_id (idexpr_id scope_none "other")) id_repr_m))) ::
-          stmt_return (expr_unop unop.deref (expr_id (idexpr_id scope_none "this"))) ::
-          nil))) in
-
-  let eq_operator :=
-    decl_fundef
-      declspec.none
-      (funtypeexpr_make
-        (typeexpr_primitive primtype.bool)
-        (make_funargs (funarg_named (cg.constref_of cls_type) "other" :: nil))
-        (fnqual.set_noexcept (fnqual.set_const fnqual.none))
-        false)
-      (idexpr_operator scope_none (overloadable_operator.binary binop.eq))
-      attrspec.none
-      (funbody_stmts cinits_nil
-        (make_stmts
-          (stmt_return
-            (expr_binop binop.eq
-              (expr_unop unop.deref (expr_id id_repr_m))
-              (expr_unop unop.deref (expr_memdot
-                (expr_id (idexpr_id scope_none "other")) id_repr_m))) ::
-          nil))) in
-
-  let repr_member_decl := (decl_simple declspec.none repr_ptr_type id_repr_m attrspec.none) in
-  let clsdecls :=
-    (make_clsdecls
-      ((clsdecl_group
-        visibility_spec.vis_public
-        (make_decls
-          (default_constructor ::
-           copy_constructor ::
-           move_constructor ::
-           assign_operator ::
-           assign_move_operator ::
-           eq_operator ::
-           factory_fns ++
-           match_fn_tpldecl ::
-           nil))) ::
-      (clsdecl_group
-        visibility_spec.vis_private
-        (make_decls (
-          repr_base_class_def ::
-          repr_classes ++
-          primary_constructor ::
-          repr_member_decl ::
-          nil))) ::
-      nil)) in
-  (tpl, cls_id, clsdecls).
-
-Definition one_inductive_decl (oi : one_inductive.t) : decl_t :=
-  let (x, clsdecls) := one_inductive_decl_parts oi in
-  let (tplargs, cls_id) := x in
-  maybe_template tplargs (decl_class cls_id true clsinherits_nil clsdecls).
 
 (* If a decl_t is actually a definition of something, turn this into
 a (forward) declaration of the object. This can be either variables,
@@ -845,6 +279,603 @@ Definition generate_stripped_class_def
     : decl_t :=
   (maybe_template tplargs (decl_class id true clsinherits_nil (clsdecls_remove_defs decls))).
 
+Module env.
+  Inductive t : Set :=
+    | empty : t.
+
+  Fixpoint to_type (e : expr.t) (this : t) : typeexpr_t :=
+    match e with
+      | expr.global n => cg.named_type n
+      | expr.local n _ => cg.named_type n
+      | expr.app fn arg =>
+        to_type_template_apply fn ((to_type arg this) :: nil) this
+      | expr.product argname argtype body =>
+        to_type_fn_abstract ((argname, to_type argtype this) :: nil) body this
+    end
+  with to_type_template_apply (fn : expr.t) (args : list typeexpr_t) (this : t) : typeexpr_t :=
+    match fn with
+      | expr.global n =>
+        let tplargs := from_list (map (fun arg => tplarg_type arg) args) in
+        typeexpr_id (idexpr_template scope_none (templateid_make n tplargs))
+      | expr.app fn arg =>
+        to_type_template_apply fn (args ++ (to_type arg this) :: nil) this
+      | _ => typeexpr_primitive (primtype.auto)
+    end
+  with to_type_fn_abstract (args : list (option string * typeexpr_t)) (body : expr.t) (this : t) : typeexpr_t :=
+    match body with
+      | expr.product argname argtype body =>
+        to_type_fn_abstract (args ++ ((argname, to_type argtype this) :: nil)) body this
+      | expr.global n =>
+        let result_type := cg.named_type n in
+        cg.fn_type result_type args
+      | expr.local n _ =>
+        let result_type := cg.named_type n in
+        cg.fn_type result_type args
+      | expr.app fn arg =>
+        let result_type := to_type_template_apply fn ((to_type arg this) :: nil) this in
+        cg.fn_type result_type args
+    end.
+  Definition to_tplformarg (name : string) (e : expr.t) (this : t) : tplformarg_t :=
+    match e with
+      | expr.global ename =>
+        if string_dec ename "Set" then
+          tplformarg_typename name
+        else if string_dec ename "Type" then
+          tplformarg_typename name
+        else
+          tplformarg_value (to_type e this) name
+      | _ => tplformarg_value (to_type e this) name
+    end.
+End env.
+
+Definition product_unfold (e : expr.t) : list (option string * expr.t) * expr.t :=
+  let head := nil in
+  (fix loop (e : expr.t) (head : list (option string * expr.t))
+      : list (option string * expr.t) * expr.t :=
+    match e with
+      | expr.product argname argtype body =>
+        let head := head ++ (argname, argtype) :: nil in
+        loop body head
+      | _ =>
+        (head, e)
+    end) e head.
+
+(* make choice of prefix name configurable *)
+Definition product_named_unfold (e : expr.t) : list (string * expr.t) * expr.t :=
+  let head := nil in
+  let index := 0 in
+  (fix loop (e : expr.t) (index : nat) (head : list (string * expr.t))
+      : list (string * expr.t) * expr.t :=
+    match e with
+      | expr.product argname argtype body =>
+        let name :=
+          match argname with
+            | Some name => name
+            | None => ("x" ++ (string_of_nat index))%string
+          end in
+        let head := head ++ (name, argtype) :: nil in
+        loop body (S index) head
+      | _ =>
+        (head, e)
+    end) e index head.
+
+Fixpoint collect_tplformargs_from_product
+    (e : expr.t) : tplformargs_t :=
+  match e with
+    | expr.product maybe_name argtype body =>
+      let name :=
+        match maybe_name with
+          | Some name => name
+          | None => "T"%string
+        end in
+      tplformargs_cons (tplformarg_typename name) (collect_tplformargs_from_product body)
+    | _ => tplformargs_nil
+  end.
+
+
+(*** INDUCTIVE XFORM CODE ***)
+
+Definition one_inductive_fwd (oi : one_inductive.t) : decl_t :=
+  let (name, sig, constructors) := oi in
+  let tpl := collect_tplformargs_from_product sig in
+  let d := decl_class_fwd (idexpr_id scope_none name) in
+  maybe_template tpl d.
+
+Definition inductive_fwd (i : inductive.t) : list decl_t :=
+  let (ois) := i in
+  map (one_inductive_fwd) ois.
+
+Definition gen_virtual_destructor_decldef (name : string) : decl_t :=
+  let ds := declspec.none in
+  let ds := declspec.set_virtual ds in
+  decl_consdesdef
+    ds
+    (idexpr_destructor scope_none name)
+    (from_list nil)
+    fnqual.none
+    attrspec.none
+    (funbody_stmts cinits_nil (from_list nil)).
+
+Definition make_repr_base_class (name : string) :=
+  let repr_cls_type := typeexpr_id (idexpr_id scope_none name) in
+  let eq_operator :=
+    decl_fundef
+      (declspec.set_virtual declspec.none)
+      (funtypeexpr_make
+        (typeexpr_primitive primtype.bool)
+        (from_list (funarg_named (cg.constref_of repr_cls_type) "other" :: nil))
+        (fnqual.set_noexcept (fnqual.set_const fnqual.none))
+        false)
+      (idexpr_operator scope_none (overloadable_operator.binary binop.eq))
+      attrspec.none
+      funbody_abstract in
+  decl_class
+    (idexpr_id scope_none name)
+    false
+    (from_list nil)
+    (clsdecls_cons
+      (clsdecl_group
+        visibility_spec.vis_public
+        (from_list
+          (gen_virtual_destructor_decldef name ::
+          eq_operator ::
+          nil)))
+      (from_list nil)).
+
+Definition constructor_reprclass_name (cons : inductive_constructor.t) : string :=
+  ((inductive_constructor.name cons) ++ "_repr").
+
+Definition constructor_reprclass_members (cons : inductive_constructor.t)
+    : list (string * expr.t) :=
+  fst (product_named_unfold (inductive_constructor.type cons)).
+
+Fixpoint make_cinits (is : list cinit_t)
+    : cinits_t :=
+  match is with
+    | nil => cinits_nil
+    | cons i is => cinits_cons i (make_cinits is)
+  end.
+
+Definition make_constructor_repr_class
+    (cons : inductive_constructor.t)
+    (environ : env.t) :=
+  let name := constructor_reprclass_name cons in
+  let members := constructor_reprclass_members cons in
+
+  let repr_cls_id := idexpr_id scope_none name in
+  let repr_cls_type := typeexpr_id repr_cls_id in
+  let repr_constptr := typeexpr_pointer (typeexpr_const repr_cls_type) in
+
+  let base_cls_id := (idexpr_id scope_none "repr_base") in
+  let base_cls_type := typeexpr_id base_cls_id in
+
+  let member_decls := map
+    (fun (mem : string * expr.t) =>
+      let (name, e) := mem in
+      let type := env.to_type e environ in
+      decl_simple declspec.none type (idexpr_id scope_none name) attrspec.none) members in
+  let init_formal_args := map
+    (fun (mem : string * expr.t) =>
+      let (name, e) := mem in
+      let type := env.to_type e environ in
+      funarg_named type (name ++ "_init")) members in
+  let initializers := map
+    (fun (mem : string * expr.t) =>
+      let (name, e) := mem in
+      cinit_make
+        (idexpr_id scope_none name)
+        (cg.move_of (expr_id (idexpr_id scope_none (name ++ "_init"))))) members in
+  let cls_constructor := decl_consdesdef
+    declspec.none
+    (idexpr_id scope_none name)
+    (from_list init_formal_args)
+    fnqual.none
+    attrspec.none
+    (funbody_stmts
+      (make_cinits initializers)
+      stmts_nil) in
+  let overridden_eq_operator :=
+    decl_fundef
+      declspec.none
+      (funtypeexpr_make
+        (typeexpr_primitive primtype.bool)
+        (from_list (funarg_named (cg.constref_of base_cls_type) "other" :: nil))
+        (fnqual.set_noexcept (fnqual.set_const fnqual.none))
+        false)
+      (idexpr_operator scope_none (overloadable_operator.binary binop.eq))
+      (attrspec.set_override attrspec.none)
+      (funbody_stmts (from_list nil)
+        (from_list
+          (stmt_ifelse
+            (condition_decl
+              declspec.none (typeexpr_primitive primtype.auto)
+              (idexpr_id scope_none "spec")
+              attrspec.none
+              (expr_dynamic_cast repr_constptr (expr_unop unop.address_of (expr_id (idexpr_id scope_none "other")))))
+            (stmt_block (from_list
+              (stmt_return (expr_binop binop.eq
+                (expr_unop unop.deref (expr_id (idexpr_id scope_none "this")))
+                (expr_unop unop.deref (expr_id (idexpr_id scope_none "spec"))))
+              :: nil)))
+            (stmt_block (from_list
+              (stmt_return (expr_id (idexpr_id scope_none "false")) :: nil))) ::
+          nil))) in
+  let member_compare := map
+    (fun (mem : string * expr.t) =>
+      let (name, e) := mem in
+      let id := idexpr_id scope_none name in
+      expr_binop binop.eq (expr_id id) (expr_memdot (expr_id (idexpr_id scope_none "other")) id))
+      members in
+  let all_member_eq := fold_right
+    (fun (x y : expr_t) => expr_binop binop.logic_and x y)
+    (expr_id (idexpr_id scope_none "true")) member_compare in
+  let specialized_eq_operator :=
+    decl_fundef
+      declspec.none
+      (funtypeexpr_make
+        (typeexpr_primitive primtype.bool)
+        (from_list (funarg_named (cg.constref_of repr_cls_type) "other" :: nil))
+        (fnqual.set_noexcept (fnqual.set_const fnqual.none))
+        false)
+      (idexpr_operator scope_none (overloadable_operator.binary binop.eq))
+      attrspec.none
+      (funbody_stmts cinits_nil
+        (from_list (stmt_return all_member_eq :: nil))) in
+  decl_class
+    repr_cls_id
+    true
+    (clsinherits_cons (clsinherit_single false visibility_spec.vis_public base_cls_id) clsinherits_nil)
+    (from_list
+      ((clsdecl_group
+        visibility_spec.vis_public
+        (from_list (cls_constructor :: specialized_eq_operator :: overridden_eq_operator :: member_decls))) :: nil)).
+
+(*
+  Roughly builds the following:
+
+  if (const as_type* temp_name = dynamic_cast<const as_type*>(base_expr)) {
+    call_expr(temp_name->member1, temp_name->member2, ..., temp_name->membern);
+  }
+
+  Returns the "condition" and "body" part of the if statement as a pair.
+
+  Can form the above statement as:
+    stmt_if condition body
+*)
+Definition make_single_match_test
+    (base_expr : expr_t) (as_type : typeexpr_t) (temp_name : idexpr_t)
+    (call_expr : expr_t) (members : list string)
+    : condition_t * stmt_t :=
+  let target_type := cg.constptr_of as_type in
+  let temp_expr := expr_id temp_name in
+  let callargs :=
+    map
+      (fun member =>
+        expr_memarrow (expr_id temp_name) (idexpr_id scope_none member))
+      members in
+  let cond := (condition_decl
+      declspec.none (cg.type_auto) temp_name attrspec.none
+      (expr_dynamic_cast target_type base_expr)) in
+  let body :=
+    stmt_block (
+      from_list
+        ((stmt_return (expr_call call_expr (from_list callargs))) :: nil)) in
+  (cond, body).
+
+(*
+  Produce a statement that checks 'base_expr' with match for any of the
+  constructor repr classes (via dynamic_cast) and dispatches to the
+  corresponding call expression.
+*)
+Fixpoint make_match_constructors
+    (base_expr : expr_t) (branches : list (inductive_constructor.t * expr_t))
+    : stmt_t :=
+  match branches with
+    | nil => stmt_block (from_list (stmt_expr (cg.throw_logic_error "impossible case" ) :: nil))
+    | branch :: branches =>
+      let sub := make_match_constructors base_expr branches in
+      let (cons, call_expr) := branch in
+      let cons_name := constructor_reprclass_name cons in
+      let cons_members := constructor_reprclass_members cons in
+      let member_names := map fst cons_members in
+      let as_type := typeexpr_id (idexpr_id scope_none cons_name) in
+      let temp_name := idexpr_id scope_none "tmp" in
+      let (cond, body) := make_single_match_test base_expr as_type temp_name call_expr member_names in
+      stmt_ifelse cond body sub
+  end.
+
+Definition make_name_type_pairs (args : list (option string * expr.t)) (environ : env.t)
+    : list (string * typeexpr_t) :=
+  map
+    (fun (ca : option string * expr.t) =>
+      let (n, e) := ca in
+      let type := env.to_type e environ in
+      let name := match n with
+        | Some n => n
+        | None => "_"%string
+      end in
+      (name, type))
+    args.
+
+Definition make_match_fntype
+    (constructors : list inductive_constructor.t)
+    (environ : env.t) : (list tplformarg_t) * funtypeexpr_t :=
+  (* special case for empty inductive type (not useful, but...) *)
+  match constructors with
+    | first_constructor :: _ =>
+      (* collect names of all constructors *)
+      let consnames := map inductive_constructor.name constructors in
+      (* template argument list for match handler functionals *)
+      let tplargs := map (fun name => tplformarg_typename ("F" ++ name)%string) consnames in
+      (* the formal arguments of our "match" function *)
+      let formal_args :=
+        from_list (
+          map
+            (fun name =>
+             funarg_named
+              (cg.constref_of (cg.named_type ("F" ++ name)))
+              ("f" ++ name))
+            consnames) in
+      (* arguments to first constructor *)
+      let pre_callargs := fst (product_unfold (inductive_constructor.type first_constructor)) in
+      (* turn them into "declval" constructs *)
+      let callargs := map (fun (ca : option string * expr.t) =>
+        let (_, e) := ca in
+        let type := env.to_type e environ in
+        cg.declval_of (cg.constref_of type)) pre_callargs in
+      let ret_type :=
+        typeexpr_decltype (expr_call (expr_id (idexpr_id scope_none ("F" ++ (inductive_constructor.name first_constructor)))) (from_list callargs)) in
+      (tplargs, funtypeexpr_make ret_type formal_args fnqual.none true)
+    | nil =>
+      (nil, funtypeexpr_make (typeexpr_primitive primtype.void) funargs_nil fnqual.none false)
+  end.
+
+Definition make_inductive_cons_factory_fn
+    (ind_clsname : string) (consname : string) (cons_args : list (string * expr.t))
+    : decl_t :=
+  let environ := env.empty in
+  let formal_args :=
+    map
+      (fun (c : string * expr.t) =>
+        let (name, e) := c in
+        funarg_named (env.to_type e environ) name)
+      cons_args in
+  let args :=
+    map
+      (fun (c : string * expr.t) =>
+        let (name, e) := c in
+        cg.move_of (expr_id (idexpr_id scope_none name)))
+      cons_args in
+  let fntype :=
+    funtypeexpr_make
+      (cg.named_type ind_clsname)
+      (from_list formal_args)
+      fnqual.none
+      false in
+  let repr_instance :=
+    cg.make_shared_of
+      (cg.named_type (consname ++ "_repr"))
+      args in
+  let cls_instance :=
+    expr_call (expr_id (idexpr_id scope_none ind_clsname)) (from_list (repr_instance :: nil)) in
+  decl_fundef
+    (declspec.set_static declspec.none)
+    fntype
+    (idexpr_id scope_none consname)
+    attrspec.none
+    (funbody_stmts
+      cinits_nil
+      (from_list (stmt_return cls_instance :: nil))).
+
+Module oind_cpp_repr.
+  Inductive t : Set :=
+    | make :
+      forall (tpl : tplformargs_t),
+      forall (clsid : idexpr_t),
+      forall (clsdecls : clsdecls_t),
+      t.
+End oind_cpp_repr.
+
+Module ind_cpp_repr.
+  Definition t := list oind_cpp_repr.t.
+End ind_cpp_repr.
+
+Definition oind_convert (oi : one_inductive.t)
+    : oind_cpp_repr.t :=
+  let environ := env.empty in
+  let (name, sig, constructors) := oi in
+
+  (* names of the inductive constructors *)
+  let consnames := map (fun (c : inductive_constructor.t) => let (name, _) := c in name) constructors in
+
+  (* template arguments, in case this is a parameterized inductive type *)
+  let tpl := collect_tplformargs_from_product sig in
+
+  (* the C++ class name... *)
+  let cls_name := name in
+  let cls_id := idexpr_id scope_none cls_name in
+  let cls_type := typeexpr_id cls_id in
+
+  (* the repr_ member id *)
+  let id_repr_m := (idexpr_id scope_none "repr_") in
+
+  (* internal base representation class, abstract *)
+  let repr_base_class_def := make_repr_base_class "repr_base" in
+  let repr_ptr_type := (cg.shared_ptr_of (cg.named_type "repr_base")) in
+
+  (* internal representation classes, to represent the different
+  inductive constructors *)
+  let repr_classes := map (fun c => make_constructor_repr_class c environ) constructors in
+
+  (* match function to discriminate between the different constructors *)
+  let (match_fn_tplargs, match_fn_type) := make_match_fntype constructors environ in
+  let cons_call := map
+    (fun (cons : inductive_constructor.t) =>
+      (cons, expr_id (idexpr_id scope_none ("f" ++ inductive_constructor.name cons)))) constructors in
+  let match_fn_decl :=
+    decl_fundef
+      declspec.none
+      match_fn_type
+      (idexpr_id scope_none "match")
+      attrspec.none
+      (funbody_stmts
+        (from_list nil)
+        (from_list
+          (make_match_constructors (expr_id id_repr_m) cons_call :: nil))) in
+  let match_fn_tpldecl := maybe_template (from_list match_fn_tplargs) match_fn_decl in
+
+  (* The static factory functions to create instances of this object
+  per each inductive constructor. *)
+  let factory_fns :=
+    map
+      (fun (cons : inductive_constructor.t) =>
+        let (consname, _) := cons in
+        let members := constructor_reprclass_members cons in
+        make_inductive_cons_factory_fn cls_name consname members
+      )
+      constructors in
+
+  (* C++ class constructors *)
+  let primary_constructor :=
+    decl_consdesdef
+      (declspec.set_explicit declspec.none)
+      cls_id
+      (from_list ((funarg_named repr_ptr_type "repr") :: nil))
+      (fnqual.set_noexcept fnqual.none)
+      attrspec.none
+      (funbody_stmts
+        (cinits_cons (cinit_make (idexpr_id scope_none "repr_") (cg.move_of (expr_id (idexpr_id scope_none "repr")))) cinits_nil)
+        (from_list nil)) in
+  let copy_constructor :=
+    decl_consdesdef
+      declspec.none
+      cls_id
+      (from_list (((funarg_named (cg.constref_of cls_type) "other")) :: nil))
+      (fnqual.set_noexcept fnqual.none)
+      attrspec.none
+      funbody_default in
+  let move_constructor :=
+    decl_consdesdef
+      declspec.none
+      cls_id
+      (from_list (((funarg_named (typeexpr_rvaluereference cls_type) "other")) :: nil))
+      (fnqual.set_noexcept fnqual.none)
+      attrspec.none
+      funbody_default in
+  let default_constructor := cg.deleted_constructor cls_name nil in
+
+  let assign_operator :=
+    decl_fundef
+      declspec.none
+      (funtypeexpr_make
+        (typeexpr_reference cls_type)
+        (from_list (funarg_named (cg.constref_of cls_type) "other" :: nil))
+        (fnqual.set_noexcept fnqual.none)
+        false)
+      (idexpr_operator scope_none (overloadable_operator.binary binop.assign))
+      attrspec.none
+      (funbody_stmts
+        (from_list nil)
+        (from_list (
+          stmt_expr (expr_binop binop.assign (expr_id id_repr_m)
+            (expr_memarrow (expr_id (idexpr_id scope_none "other")) id_repr_m)) ::
+          stmt_return (expr_unop unop.deref (expr_id (idexpr_id scope_none "this"))) ::
+          nil))) in
+
+  let assign_move_operator :=
+    decl_fundef
+      declspec.none
+      (funtypeexpr_make
+        (typeexpr_reference cls_type)
+        (from_list (funarg_named (typeexpr_rvaluereference cls_type) "other" :: nil))
+        (fnqual.set_noexcept fnqual.none)
+        false)
+      (idexpr_operator scope_none (overloadable_operator.binary binop.assign))
+      attrspec.none
+      (funbody_stmts
+        (from_list nil)
+        (from_list (
+          stmt_expr (expr_binop binop.assign (expr_id id_repr_m)
+            (cg.move_of (expr_memarrow (expr_id (idexpr_id scope_none "other")) id_repr_m))) ::
+          stmt_return (expr_unop unop.deref (expr_id (idexpr_id scope_none "this"))) ::
+          nil))) in
+
+  let eq_operator :=
+    decl_fundef
+      declspec.none
+      (funtypeexpr_make
+        (typeexpr_primitive primtype.bool)
+        (from_list (funarg_named (cg.constref_of cls_type) "other" :: nil))
+        (fnqual.set_noexcept (fnqual.set_const fnqual.none))
+        false)
+      (idexpr_operator scope_none (overloadable_operator.binary binop.eq))
+      attrspec.none
+      (funbody_stmts 
+        (from_list nil)
+        (from_list
+          (stmt_return
+            (expr_binop binop.eq
+              (expr_unop unop.deref (expr_id id_repr_m))
+              (expr_unop unop.deref (expr_memdot
+                (expr_id (idexpr_id scope_none "other")) id_repr_m))) ::
+          nil))) in
+
+  let repr_member_decl := (decl_simple declspec.none repr_ptr_type id_repr_m attrspec.none) in
+  let clsdecls :=
+    (from_list
+      ((clsdecl_group
+        visibility_spec.vis_public
+        (from_list
+          (default_constructor ::
+           copy_constructor ::
+           move_constructor ::
+           assign_operator ::
+           assign_move_operator ::
+           eq_operator ::
+           factory_fns ++
+           match_fn_tpldecl ::
+           nil))) ::
+      (clsdecl_group
+        visibility_spec.vis_private
+        (from_list (
+          repr_base_class_def ::
+          repr_classes ++
+          primary_constructor ::
+          repr_member_decl ::
+          nil))) ::
+      nil)) in
+  oind_cpp_repr.make tpl cls_id clsdecls.
+
+Definition ind_convert (i : inductive.t) : ind_cpp_repr.t :=
+  match i with
+    | inductive.make oinds =>
+      map oind_convert oinds
+  end.
+
+Definition oind_gen_clsdecl (r : oind_cpp_repr.t) : decl_t := 
+  let (tplformargs, clsid, clsdecls) := r in
+  generate_stripped_class_def tplformargs clsid clsdecls.
+
+Definition oind_gen_otherdecl (r : oind_cpp_repr.t) : decls_t :=
+  let (tplformargs, clsid, clsdecls) := r in
+  from_list (generate_member_defs tplformargs clsid clsdecls).
+
+Definition ind_gen_clsdecls (r : ind_cpp_repr.t) : decls_t :=
+  from_list (map oind_gen_clsdecl r).
+
+Definition ind_gen_otherdecl (r : ind_cpp_repr.t) : decls_t :=
+  let decls := decls_nil in
+  (fix loop (decls : decls_t) (r : list oind_cpp_repr.t) {struct r} : decls_t :=
+    match r with
+      | nil => decls
+      | cons oind r =>
+        let d := oind_gen_otherdecl oind in
+        let decls := app decls d in
+        loop decls r
+    end) decls r.
+
+(**** EXAMPLES ****)
+
 Example sort_set := (expr.global "Set"%string).
 
 Example oiX :=
@@ -860,39 +891,31 @@ Example oiX :=
         (expr.app (expr.global "X"%string) (expr.local "T"%string 1))) ::
     nil).
 
+Example oiY :=
+  one_inductive.make "Y" (expr.product (Some "T"%string) sort_set sort_set) (
+    (* constructors *)
+    inductive_constructor.make "Y0"
+      (expr.product (Some "t"%string)
+        (expr.local "T"%string 1)
+        (expr.app (expr.global "Y"%string) (expr.local "T"%string 1))) ::
+    inductive_constructor.make "Y1"
+      (expr.product (Some "x"%string)
+        (expr.app (expr.global "X"%string) (expr.local "T"%string 1))
+        (expr.app (expr.global "Y"%string) (expr.local "T"%string 1))) ::
+    nil).
 
-Example i1 := inductive.make (oiX :: nil).
+Example i1 := inductive.make (oiX :: oiY :: nil).
 
 Eval lazy in (collect_tplformargs_from_product (let (_, sig, _) := oiX in sig)).
 
-Eval lazy in (serialize_tokens (decls_serialize (make_decls (inductive_fwd i1)))).
+Eval lazy in (serialize_tokens (decls_serialize (from_list (inductive_fwd i1)))).
 
-Eval lazy in (serialize_tokens (decl_serialize (one_inductive_decl oiX))).
+Example icls1 := oind_convert oiX.
 
-Eval lazy in (serialize_tokens (decl_serialize (cls_remove_defs (one_inductive_decl oiX)))).
+Eval lazy in (serialize_tokens (decl_serialize (oind_gen_clsdecl icls1))).
+Eval lazy in (serialize_tokens (decls_serialize (oind_gen_otherdecl icls1))).
 
-Example icls1 := one_inductive_decl_parts oiX.
+Example i := ind_convert i1.
 
-Example icls1_tplargs := fst (fst icls1).
-Example icls1_idexpr := snd (fst icls1).
-Example icls1_cdecls := snd icls1.
-
-Eval lazy in (serialize_tokens (decl_serialize (generate_stripped_class_def icls1_tplargs icls1_idexpr icls1_cdecls))).
-Eval lazy in (serialize_tokens (decls_serialize (make_decls (generate_member_defs icls1_tplargs icls1_idexpr icls1_cdecls)))).
-
-(*
-
-TODO:
-
-- full support for mutual inductive defs
-
-DONE:
-
-+ C++ constructors of X
-+ C++ factory functions corresponding to inductive constructors
-+ C++ constructors of repr classes
-+ equality operator of X
-+ assignment operator of X
-+ un-inline from declaration
-
-*)
+Eval lazy in (serialize_tokens (decls_serialize (ind_gen_clsdecls i))).
+Eval lazy in (serialize_tokens (decls_serialize (ind_gen_otherdecl i))).
